theories/iris/logrel/module.v
@@ -1,19 +1,28 @@
 Require Import RichWasm.typing.
 Require Import RichWasm.compiler.module.
+Require Import RichWasm.iris.host.iris_host.
 Require Import RichWasm.iris.rules.iris_rules.
-Require Import RichWasm.iris.logrel.
+From RichWasm.iris Require Import logrel memory util.
 
 Set Bullet Behavior "Strict Subproofs".
 Set Default Goal Selector "!".
 
 Section Fundamental.
 
-  Context `{Σ : gFunctors}.
+  Context `{!logrel_na_invs Σ}.
+  Context `{!wasmG Σ}.
+  Context `{!richwasmG Σ}.
+  Context `{!hvisG Σ}.
+  Context `{!hmsG Σ}.
+  Context `{!hasG Σ}.
 
-  Theorem fundamental_module m m' ω :
-    has_module_type m ω ->
+  Variable rti : rt_invariant Σ.
+  Variable sr : store_runtime.
+
+  Theorem fundamental_module m m' mt :
+    has_module_type m mt ->
     run_modgen (compile_module m) mod_empty = inr (tt, m') ->
-    ⊢ @has_module_type_sem Σ m' ω.
+    ⊢ module_interp rti sr mt m'.
   Admitted.
 
 End Fundamental.
